CompilerEnv & RuntimeEnv FBounds now save the trm the intermdiate result is assigned to

Lp2lc/Active/STLC/STLCDef.lean
@@ -118,13 +118,13 @@ def eval (self : AST.Trm F) : RecOption (AST.Val F)
       match anf with
       | (.yield (some (.fn body _tIn)), .yield (some input)) =>
         -- let permission := env.canSaveAny input
-        let index := env.trm2valCtx.save input
+        let index := env.trm2valCtx.save ⟨arg, input⟩
         (body index).eval fuel
       | (.outOfFuel, _) => .outOfFuel
       | (_, .outOfFuel) => .outOfFuel
       | _ => .yield none
     | @AST.Trm.ref _ i =>
-      .yield (some (env.trm2valCtx.load i))
+      .yield (some (env.trm2valCtx.load i).val)
 
 end
 
